ModularEngine/src/LogicEngine.FStar/marshall.fst
@@ -2,6 +2,50 @@ module Marshall
 open TypeHeaders
 open Types
 
+logic function Strcat : list string -> string
+logic function ReprVar : var -> string
+logic function ReprVars : vars -> string
+logic function ReprMono : term -> string
+logic function ReprPoly : polyterm -> string
+assume forall (xs:vars) (t:term). 
+                         ReprPoly (ForallT xs t) = Strcat ["(Forall ("; 
+                                                           (ReprVars xs);
+                                                           ") ";
+                                                           (ReprMono t);
+                                                           ")"]
+assume forall (t:term). ReprPoly (MonoTerm t) = ReprMono t
+
+(* type Star :: P => * = *)
+(*  | MkStar : 'a::P -> Star 'a *)
+
+(* val rep_isa_function:  n:nat  *)
+(* (\*                     -> total n polyterm () *\) *)
+(*                     -> p:polyterm{SizeOf p = n} *)
+(*                     -> s1:string{(ReprPoly p)=s1}  *)
+(*                     -> s2:string{(ReprPoly p) = s2}  *)
+(*                     -> Star (Eq s1 s2) *)
+
+(* val rep_is_injective:   p1:polyterm  *)
+(*                      -> p2:polyterm  *)
+(*                      -> s:string{(ReprPoly p1=s) && (ReprPoly p2=s)} *)
+(*                      -> Star (Eq p1 p2) *)
+
+(* Note: these functions are recursive and so cannot be in P
+         as such, we cannot prove directly that they are total functions. 
+         If we can do this totality proof in some other way, for example, 
+         by providing an explicit ranking function, then we will have proved 
+         that at least ReprPoly is at least a function. *)
+val printInfon: p:polyterm -> b:string{(ReprPoly p)=b}
+let printInfon p = raise "TODO"
+
+(* Note: As for the printer, this function is recursive and so not in P. *)
+val parseInfon: b:string -> option (p:polyterm{(Net.Received b => Net.Received p) &&
+                                               (ReprPoly p)=b})
+let parseInfon b = raise "TODO"                                         
+
+
+(* -------------------------------------------------------------------------------- *)
+
 type message :: _ =  fun ('P::principal => principal => polyterm => E) => 
     ((pfrom:principal *
         pto:principal *
@@ -14,11 +58,6 @@ type msg =
   | Forwarded : message trivial -> msg
   | Justified : message SaysTo -> msg
 
-
-val polyterm2bytes : polyterm -> bytes
-val bytes2polyterm : bytes -> polyterm
-val parse: b:bytes -> p:polyterm{Net.Received b => Net.Received p}
 val concat : list bytes -> bytes
 val unconcat: bytes -> list bytes
-
 val msg2bytes: msg -> bytes
